\part{Basic Set Theory}

\chapter{Axioms of Set Theory}

\Exercise{1} Verify (1.1).
\begin{solution}
  If $a = c$ and $b = d$, then $(a, b) = (c, d)$ as a consequence of an axiom of 
  first-order logic with equality, namely, that equals may be substituted for
  equals in a formula.

  Conversely, suppose that $(a, b) = (c, d)$. Then
  \[
    \{ \{ a \}, \{ a, b \} \}  = \{ \{ c \}, \{ c, d \} \}.
  \]
  If $a = b$, then
  \[
    \{ \{ a \}, \{ a, b \} \} = \{ \{ a \}, \{ a, a \} \} = \{ \{ a \} \}.
  \]
Therefore $\{ a \} = \{ c \}$ and  $\{ a \} = \{ c, d \}$. Hence, $a = c = d$,
from which it follows that $a = c$ and $b = d$. If $a \neq b$, then
$\{ a \} = \{ c \}$ and $\{ a, b \} = \{ c, d \}$. Therefore $a = c$, and from
this it follows that $\{ a, b \} = \{ a, d \}$. Hence $b = d$.
\end{solution}